VLSM/Common.v
@@ -79,6 +79,12 @@ Require Import Lib.Preamble Lib.ListExtras Lib.StreamExtras.
 
     Definition protocol_message_prop (m : message) :=
       exists s : state, protocol_prop (s, (Some m)).
+    
+    Definition option_protocol_message_prop (om : option message) :=
+      match om with 
+      | None => True
+      | Some m => protocol_message_prop m
+      end.
 
     Definition protocol_state : Type :=
       { s : state | protocol_state_prop s }.
@@ -1359,10 +1365,205 @@ Require Import Lib.Preamble Lib.ListExtras Lib.StreamExtras.
 
   End VLSM_equality.
 
-  Definition pre_loaded_vlsm_sig
+  Section VLSM_incl_from_protocol_state.
+
+  Context
     {message : Type}
-    {vtype : VLSM_type message}
-    {Sig : LSM_sig vtype}
+    {T : VLSM_type message}
+    {S1 S2 : LSM_sig T}
+    (X1 : VLSM S1)
+    (X2 : VLSM S2)
+    (Hinitial_state : 
+      forall s : state,
+        @initial_state_prop _ _ S1 s -> @initial_state_prop _ _ S2 s
+    )
+    (Hprotocol_state : 
+      forall (s : state) (om : option message),
+        protocol_prop X1 (s,om) -> protocol_state_prop X2 s
+    )
+    (Hprotocol_transition :
+      forall (l : label) (is os : state) (iom oom : option message),
+        verbose_valid_protocol_transition X1 l is os iom oom
+        -> verbose_valid_protocol_transition X2 l is os iom oom
+    )
+    .
+
+  Lemma VLSM_incl_finite_ptrace
+    (s : state)
+    (ls : list in_state_out)
+    (Hpxt : finite_ptrace_from X1 s ls)
+    : finite_ptrace_from X2 s ls
+    .
+  Proof.
+    induction Hpxt.
+    - constructor.
+      destruct H as [m H].
+      apply Hprotocol_state in H. assumption.
+    - constructor; try assumption.
+      apply Hprotocol_transition. assumption.
+  Qed.
+
+  Lemma VLSM_incl_infinite_ptrace
+    (s : state)
+    (ls : Stream in_state_out)
+    (Hpxt : infinite_ptrace_from X1 s ls)
+    : infinite_ptrace_from X2 s ls
+    .
+  Proof.
+    generalize dependent ls. generalize dependent s.
+    cofix H.
+    intros s [[l input destination output] ls] Hx.
+    inversion Hx; subst.
+    specialize (H destination ls H3).
+    constructor; try assumption.
+    apply Hprotocol_transition.
+    assumption.
+  Qed.
+
+  Lemma VLSM_incl_from_protocol_state
+    : VLSM_incl X1 X2
+    .
+  Proof.
+    intros [s ls| s ss]; simpl; intros [Hxt Hinit].  
+    - apply VLSM_incl_finite_ptrace in Hxt.
+      split; try assumption.
+      apply Hinitial_state. assumption.
+    - apply VLSM_incl_infinite_ptrace in Hxt.
+      split; try assumption.
+      apply Hinitial_state. assumption.
+  Qed.
+
+  End VLSM_incl_from_protocol_state.
+
+  Section basic_VLSM_incl.
+
+  Context
+    {message : Type}
+    {T : VLSM_type message}
+    {S1 S2 : LSM_sig T}
+    (X1 : VLSM S1)
+    (X2 : VLSM S2)
+    (Hinitial_state : 
+      forall s : state,
+        @initial_state_prop _ _ S1 s -> @initial_state_prop _ _ S2 s
+    )
+    (Hprotocol_message : 
+      forall (l : label) (s : state) (om : option message),
+        @valid _ _ _ X1 l (s, om)
+        -> exists _s : state, protocol_prop X2 (_s, om)
+    )
+    (Hvalid : 
+      forall (l : label) (s : state) (om : option message),
+        @valid _ _ _ X1 l (s, om)
+        -> @valid _ _ _ X2 l (s, om)
+    )
+    (Htransition :
+      forall (l : label) (s : state) (om : option message),
+        @transition _ _ _ X1 l (s, om) = @transition _ _ _ X2 l (s, om)
+    )
+    .
+  
+  Lemma VLSM_incl_protocol_state
+    (s : state)
+    (om : option message)
+    (Hps : protocol_prop X1 (s,om))
+    : protocol_state_prop X2 s.
+  Proof.
+    remember (s, om) as som.
+    generalize dependent om. generalize dependent s.
+    induction Hps; intros; inversion Heqsom; subst; clear Heqsom.
+    - exists None.
+      unfold s in *. clear s.
+      destruct is as [is His]; simpl.
+      apply Hinitial_state in His.
+      replace is with (proj1_sig (exist _ is His)); try reflexivity.
+      apply (protocol_initial_state X2).
+    - exists None.
+      unfold s in *. clear s.
+      destruct s0 as [is His]; simpl.
+      apply Hinitial_state in His.
+      replace is with (proj1_sig (exist _ is His)); try reflexivity.
+      apply (protocol_initial_state X2).
+    - exists om0. 
+      rewrite Htransition in H0.
+      specialize (IHHps1 s _om eq_refl). destruct IHHps1 as [_omf Hfps].
+      replace (s1, om0) with (  @transition _ _ _ X2 l1 (s, om))
+      ; try assumption.
+      specialize (Hprotocol_message l1 s om Hv).
+      destruct Hprotocol_message as [_sX HpmX].
+      apply (protocol_generated X2) with _omf _sX; try assumption.
+      apply Hvalid.
+      assumption.
+  Qed.
+
+  Lemma VLSM_incl_verbose_valid_protocol_transition
+    (l : label)
+    (is os : state)
+    (iom oom : option message)
+    (Ht : verbose_valid_protocol_transition X1 l is os iom oom)
+    : verbose_valid_protocol_transition X2 l is os iom oom
+    .
+  Proof.
+    destruct Ht as [[_om Hps] [[_s Hpm] [Hv Ht]]].
+    repeat split.
+    - apply VLSM_incl_protocol_state with _om. assumption.
+    - apply Hprotocol_message in Hv. assumption.
+    - apply Hvalid. assumption.
+    - rewrite <- Htransition. assumption.
+  Qed.
+
+  Lemma basic_VLSM_incl
+    : VLSM_incl X1 X2
+    .
+  Proof.
+    apply (VLSM_incl_from_protocol_state X1 X2); try assumption.
+    - apply VLSM_incl_protocol_state.
+    - apply VLSM_incl_verbose_valid_protocol_transition.
+  Qed.
+
+  End basic_VLSM_incl.
+
+  Section VLSM_incl_from_protocol_prop.
+
+  Context
+    {message : Type}
+    {T : VLSM_type message}
+    {S1 S2 : LSM_sig T}
+    (X1 : VLSM S1)
+    (X2 : VLSM S2)
+    (Hinitial_state : 
+      forall s : state,
+        @initial_state_prop _ _ S1 s -> @initial_state_prop _ _ S2 s
+    )
+    (Hprotocol_prop : 
+      forall som : state * option message,
+        protocol_prop X1 som -> protocol_prop X2 som
+    )
+    (Hprotocol_transition :
+      forall (l : label) (is os : state) (iom oom : option message),
+        verbose_valid_protocol_transition X1 l is os iom oom
+        -> verbose_valid_protocol_transition X2 l is os iom oom
+    )
+    .
+
+  Lemma VLSM_incl_from_protocol_prop
+    : VLSM_incl X1 X2
+    .
+  Proof.
+    apply (VLSM_incl_from_protocol_state X1 X2); try assumption.
+    intros. exists om. apply Hprotocol_prop. assumption.
+  Qed.
+
+  End VLSM_incl_from_protocol_prop.
+
+  Section pre_loaded_vlsm.
+    Context
+      {message : Type}
+      {vtype : VLSM_type message}
+      {Sig : LSM_sig vtype}
+      .
+
+  Definition pre_loaded_vlsm_sig
     (X : VLSM Sig)
     : LSM_sig vtype
     :=
@@ -1373,11 +1574,9 @@ Require Import Lib.Preamble Lib.ListExtras Lib.StreamExtras.
      ; l0 := @l0 _ _ Sig
     |}.
 
+  Context (X : VLSM Sig).
+  
   Definition pre_loaded_vlsm
-    {message : Type}
-    {vtype : VLSM_type message}
-    {Sig : LSM_sig vtype}
-    (X : VLSM Sig)
     : VLSM (pre_loaded_vlsm_sig X)
     := 
     {| transition := @transition _ _ _ X
@@ -1385,34 +1584,26 @@ Require Import Lib.Preamble Lib.ListExtras Lib.StreamExtras.
     |}.
 
   Lemma pre_loaded_protocol_prop
-    {message : Type}
-    {vtype : VLSM_type message}
-    {Sig : LSM_sig vtype}
-    (X : VLSM Sig)
     (s : state)
     (om : option message)
     (Hps : protocol_prop X (s, om))
-    : protocol_prop (pre_loaded_vlsm X) (s, om).
+    : protocol_prop pre_loaded_vlsm (s, om).
   Proof.
     induction Hps.
-    - apply (protocol_initial_state (pre_loaded_vlsm X) is).
+    - apply (protocol_initial_state pre_loaded_vlsm is).
     - destruct im as [m Him]. simpl in om0. clear Him.
       assert (Him : @initial_message_prop _ _ (pre_loaded_vlsm_sig X) m)
         by exact I.
-      apply (protocol_initial_message (pre_loaded_vlsm X) (exist _ m Him)).
-    - apply (protocol_generated (pre_loaded_vlsm X)) with _om _s; assumption.
+      apply (protocol_initial_message pre_loaded_vlsm (exist _ m Him)).
+    - apply (protocol_generated pre_loaded_vlsm) with _om _s; assumption.
   Qed.
 
   Lemma pre_loaded_verbose_valid_protocol_transition
-    {message : Type}
-    {vtype : VLSM_type message}
-    {Sig : LSM_sig vtype}
-    (X : VLSM Sig)
     (l : label)
     (is os : state)
     (iom oom : option message)
     (Ht : verbose_valid_protocol_transition X l is os iom oom)
-    : verbose_valid_protocol_transition (pre_loaded_vlsm X) l is os iom oom
+    : verbose_valid_protocol_transition pre_loaded_vlsm l is os iom oom
     .
   Proof.
     destruct Ht as [[_om Hps] [[_s Hpm] [Hv Ht]]].
@@ -1421,61 +1612,14 @@ Require Import Lib.Preamble Lib.ListExtras Lib.StreamExtras.
     - exists _s. apply pre_loaded_protocol_prop. assumption.
   Qed.
 
-  Lemma pre_loaded_finite_ptrace
-    {message : Type}
-    {vtype : VLSM_type message}
-    {Sig : LSM_sig vtype}
-    (X : VLSM Sig)
-    (s : state)
-    (ls : list in_state_out)
-    (Hpxt : finite_ptrace_from X s ls)
-    : finite_ptrace_from (pre_loaded_vlsm X) s ls
-    .
-  Proof.
-    induction Hpxt.
-    - constructor.
-      destruct H as [m H].
-      apply pre_loaded_protocol_prop in H.
-      exists m. assumption.
-    - constructor; try assumption.
-      apply pre_loaded_verbose_valid_protocol_transition. assumption.
-  Qed.
-
-  Lemma pre_loaded_infinite_ptrace
-    {message : Type}
-    {vtype : VLSM_type message}
-    {Sig : LSM_sig vtype}
-    (X : VLSM Sig)
-    (s : state)
-    (ls : Stream in_state_out)
-    (Hpxt : infinite_ptrace_from X s ls)
-    : infinite_ptrace_from (pre_loaded_vlsm X) s ls
-    .
-  Proof.
-    generalize dependent ls. generalize dependent s.
-    cofix H.
-    intros s [[l input destination output] ls] Hx.
-    inversion Hx; subst.
-    specialize (H destination ls H3).
-    constructor; try assumption.
-    apply pre_loaded_verbose_valid_protocol_transition.
-    assumption.
-  Qed.
-
   Lemma vlsm_incl_pre_loaded_vlsm
-    {message : Type}
-    {vtype : VLSM_type message}
-    {Sig : LSM_sig vtype}
-    (X : VLSM Sig)
-    (PreLoaded := pre_loaded_vlsm X)
-    : VLSM_incl X PreLoaded
+    : VLSM_incl X pre_loaded_vlsm
     .
   Proof.
-    intros [s ls| s ss]; simpl; intros [Hxt Hinit].  
-    - apply pre_loaded_finite_ptrace in Hxt.
-      split; try assumption.
-    - apply pre_loaded_infinite_ptrace in Hxt.
-      split; try assumption.
+    apply (VLSM_incl_from_protocol_prop X pre_loaded_vlsm).
+    - intros; assumption.
+    - intros [s om]. apply pre_loaded_protocol_prop.
+    - apply pre_loaded_verbose_valid_protocol_transition.
   Qed.
 
-  
+End pre_loaded_vlsm.
